Wavelet/Determinancy.lean
@@ -1,0 +1,195 @@
+import Wavelet.Semantics
+import Wavelet.Seq
+import Wavelet.Dataflow
+import Wavelet.Compile
+
+/-! Reasoning about the determinancy of semantics. -/
+
+namespace Wavelet.Semantics
+
+open Semantics
+
+abbrev CompatRel V := ∀ {n m}, Vector V n → Vector V m → Prop
+
+/-- Any yielding transitions from the same state commute,
+if a certain compatibility constraint holds on the inputs. -/
+def CommYields
+  [Arity Op]
+  (Compat : CompatRel V)
+  (sem : Semantics Op V m n)
+  : Prop :=
+  ∀ s s₁ s₂
+    op₁ inputs₁ outputs₁
+    op₂ inputs₂ outputs₂,
+    sem.lts.Step s (.yield op₁ inputs₁ outputs₁) s₁ →
+    sem.lts.Step s (.yield op₂ inputs₂ outputs₂) s₂ →
+    Compat inputs₁ inputs₂ →
+    ∃ s',
+      sem.lts.Step s₁ (.yield op₂ inputs₂ outputs₂) s' ∧
+      sem.lts.Step s₂ (.yield op₁ inputs₁ outputs₁) s'
+
+def OpInterp.Determinant
+  [Arity Op]
+  (Compat : CompatRel V)
+  (interp : OpInterp Op V)
+  : Prop :=
+  ∀ s s₁ s₂
+    op₁ inputs₁ outputs₁
+    op₂ inputs₂ outputs₂,
+    interp.interp op₁ inputs₁ s outputs₁ s₁ →
+    interp.interp op₂ inputs₂ s outputs₂ s₂ →
+    Compat inputs₁ inputs₂ →
+    ∃ s',
+      interp.interp op₁ inputs₁ s₂ outputs₁ s' ∧
+      interp.interp op₂ inputs₂ s₁ outputs₂ s'
+
+/-
+Three pieces:
+- A state invariant `P : S → Prop` on each semantics
+- A guarded transition that enforces the invariant on the base transition
+- Proof obligations
+  - Simulation between guarded transitions
+  - Invariant implies compatibility relation of values (obligation of the semantics)
+  - Compatibility relation implies commutative operators (obligation of op interp)
+  - Typing in Seq implies progress in the guarded transition
+
+Maybe just specialize to PCMs?
+
+class WithToken V where
+  token : V → PCM
+
+State invariant on Seq: for any two values v₁ v₂ in the config, token v₁ ⊥ token v₂
+-/
+
+inductive GuardedLts {S} (Inv : S → Prop) (lts : Lts S E) : Lts S E where
+  | step : Inv s → Inv s' → lts.Step s e s' → GuardedLts Inv lts s e s'
+
+/-- Guard the transition of a semantics with the given invariant. -/
+def guard [Arity Op]
+  (sem : Semantics Op V m n)
+  (Inv : sem.S → Prop) : Semantics Op V m n :=
+  {
+    S := sem.S,
+    init := sem.init,
+    lts := GuardedLts Inv sem.lts,
+    -- TODO: this is actually not true,
+    -- maybe remove this requirement?
+    yields_functional := sorry
+  }
+
+class PCM (C : Type u) where
+  add : C → C → C
+  zero : C
+  valid : C → Prop
+  eq : C → C → Prop
+
+infixl:60 " ⬝ " => PCM.add
+infix:50 " ≡ " => PCM.eq
+prefix:40 "✓ " => PCM.valid
+
+def PCM.disjoint {C : Type u} [PCM C] (a b : C) : Prop := ✓ a ⬝ b
+
+/-- TODO: Implement some type class for partial order. -/
+def PCM.le {C : Type u} [PCM C] (a b : C) : Prop := ∃ c, b ≡ a ⬝ c
+
+def PCM.framePreserving {C : Type u} [PCM C] (a b : C) : Prop :=
+  ∀ c, ✓ a ⬝ c → ✓ b ⬝ c
+
+infix:50 " ⊥ " => PCM.disjoint
+infix:50 " ≤ " => PCM.le
+infix:50 " ⟹ " => PCM.framePreserving
+
+class LawfulPCM (R : Type u) [inst : PCM R] where
+  add_comm : ∀ a b : R, a ⬝ b ≡ b ⬝ a
+  add_assoc : ∀ a b c : R, (a ⬝ b) ⬝ c ≡ a ⬝ (b ⬝ c)
+  add_ident : ∀ a : R, a ⬝ inst.zero ≡ a
+  valid_add : ∀ a b : R, ✓ a ⬝ b → ✓ a
+  valid_zero : ✓ inst.zero
+  valid_eq : ∀ a b : R, a ≡ b → ✓ a → ✓ b
+  eq_refl : ∀ a : R, a ≡ a
+  eq_symm : ∀ a b : R, a ≡ b → b ≡ a
+  eq_trans : ∀ a b c : R, a ≡ b → b ≡ c → a ≡ c
+
+/-- Uses only the LHS `InterpConsts` of a sum for constants. -/
+instance instInterpConstsSum [left : InterpConsts V] : InterpConsts (V ⊕ V') where
+  junkVal := .inl (left.junkVal)
+  toBool
+    | .inl v => left.toBool v
+    | .inr _ => none
+  fromBool := .inl ∘ left.fromBool
+  unique_fromBool_toBool b := left.unique_fromBool_toBool b
+  unique_toBool_fromBool b v hv := by
+    split at hv
+    · rename_i v'
+      have := left.unique_toBool_fromBool b v' hv
+      simp [this]
+    · contradiction
+
+end Wavelet.Semantics
+
+namespace Wavelet.Seq
+
+open Semantics Compile
+
+def Config.DisjointTokens
+  [Arity Op] [PCM T]
+  (c : Config Op χ (V ⊕ T) m n) : Prop :=
+  ∀ x₁ x₂ t₁ t₂,
+    x₁ ≠ x₂ →
+    c.vars.getVar x₁ = some (.inr t₁) →
+    c.vars.getVar x₂ = some (.inr t₂) →
+    t₁ ⊥ t₂
+
+end Wavelet.Seq
+
+namespace Wavelet.Dataflow
+
+open Semantics
+
+def Config.DisjointTokens
+  [Arity Op] [PCM T]
+  (c : Config Op χ (V ⊕ T) m n) : Prop :=
+  ∀ x₁ x₂
+    (buf₁ buf₂ : List (V ⊕ T))
+    (i : Fin buf₁.length) (j : Fin buf₂.length)
+    t₁ t₂,
+    x₁ ≠ x₂ ∨ i.val ≠ j.val →
+    c.chans x₁ = some buf₁ →
+    c.chans x₂ = some buf₂ →
+    buf₁[i] = .inr t₁ →
+    buf₂[j] = .inr t₂ →
+    t₁ ⊥ t₂
+
+end Wavelet.Dataflow
+
+namespace Wavelet.Compile
+
+open Semantics Seq Dataflow
+
+theorem sim_compile_fn'
+  [Arity Op]
+  [InterpConsts V]
+  [PCM T]
+  [DecidableEq χ]
+  (fn : Fn Op χ (V ⊕ T) m n)
+  (hnz : m > 0 ∧ n > 0)
+  (hwf : fn.AffineVar) :
+  fn.semantics.guard (Config.DisjointTokens)
+    ≲ᵣ (compileFn hnz fn).semantics.guard (Config.DisjointTokens)
+  := sorry
+
+-- theorem fn_progress
+--   [Arity Op]
+--   [InterpConsts V]
+--   [WithToken V T]
+--   [PCM T]
+--   [DecidableEq χ]
+--   (fn : Fn Op χ V m n)
+--   (hnz : m > 0 ∧ n > 0)
+--   (hwf : fn.AffineVar)
+--   (hwell_typed : sorry) :
+--   fn.semantics -- Maybe even add the tokens here?
+--     ≲ᵣ fn.semantics.guard (Config.DisjointTokens T)
+--   := sorry
+
+end Wavelet.Compile
