Wavelet/Semantics.lean
@@ -2,6 +2,5 @@ import Wavelet.Semantics.Defs
 import Wavelet.Semantics.Lts
 import Wavelet.Semantics.Link
 import Wavelet.Semantics.OpInterp
-import Wavelet.Semantics.Determinancy
 
 /-! Common definitions for semantics. -/
